cleanup code with inductive type with list of

harrison.v
@@ -1,8 +1,8 @@
 Require Import List.
 Require Import String.
 
-Open Local Scope string_scope.
-Open Local Scope list_scope.
+Open Scope string_scope.
+Open Scope list_scope.
 
 (*****************************************)
 
@@ -13,164 +13,236 @@ Record InhabitedType : Type := {
 
 (*****************************************)
 
+
 Inductive term: Set :=
 | var: string -> term
-| fct: string -> list_term -> term
-  with
-  list_term : Set :=
-| nil_term: list_term
-| cons_term: term -> list_term -> list_term.
+| fn: string -> list term -> term.
 
-Program Fixpoint term_dec (t1 t2: term): {t1 = t2} + {t1 <> t2} :=
-  match t1, t2 with
-  | var s1, var s2 => _
-  | fct f1 args1, fct f2 args2 =>
-    match string_dec f1 f2 with
-    | right _ => _
-    | left _ =>
-      match list_term_dec args1 args2 with
-      | right _ => _
-      | left _ => _
-      end
-    end
-  | var _, fct _ _ => _
-  | fct _ _, var _ => _
-  end
-with
-list_term_dec (l1 l2: list_term): {l1 = l2} + {l1 <> l2} :=
-  match l1, l2 with
-  | nil_term, nil_term => _
-  | cons_term hd1 tl1, cons_term hd2 tl2 =>
-    match term_dec hd1 hd2 with
-    | left _ =>
-      match list_term_dec tl1 tl2 with
-      | left _ => _
-      | right _ => _
-      end
-    | right _ => _
-    end
-  | nil_term, cons_term hd tl => _
-  | cons_term hd tl, nil_term => _
+(* now because we have list of term inside of term definition, we need to redefine our own induction scheme *)
+
+Fixpoint sum_list_nat (l: list nat) : nat :=
+  match l with
+  | nil => 0
+  | hd::tl => hd + sum_list_nat tl
   end.
-Next Obligation.
-  left; congruence.
-Defined.
-Next Obligation.
-  left; congruence.
-Defined.
-Next Obligation.
-  right; congruence.
-Defined.
-Next Obligation.
-  right; congruence.
-Defined.
-Next Obligation.
-  right; congruence.
-Defined.
-Next Obligation.
-  right; congruence.
-Defined.
-Next Obligation.
-  destruct (string_dec s1 s2).
-  left; congruence.
-  right; congruence.
-Defined.
-Next Obligation.
-  right; congruence.
-Defined.
-Next Obligation.
-  right; congruence.
-Defined.
-Next Obligation.
-  left; congruence.
-Defined.
-Next Obligation.
-  right; congruence.
-Defined.
-Next Obligation.
-  right; congruence.
-Defined.
 
-Fixpoint term_semantics
-         {Value: InhabitedType}
-         (ctxt_var: string -> Value)
-         (ctxt_fct: string -> list Value -> Value)
-         (t: term): Value :=
+Require Import Omega.
+
+Lemma sum_list_nat_elt: forall (l: list nat) (x: nat),
+    In x l -> sum_list_nat l >= x.
+  induction l; simpl; intros; intuition.
+  generalize (IHl _ H0); intros; intuition.
+Qed.
+
+Fixpoint term_measure (t: term): nat :=
   match t with
-  | var x => ctxt_var x
-  | fct f args => ctxt_fct f (list_term_semantics ctxt_var ctxt_fct args)
-  end
-with
-list_term_semantics
-  {Value: InhabitedType}
-  (ctxt_var: string -> Value)
-  (ctxt_fct: string -> list Value -> Value)
-  (lt: list_term): list Value :=
-  match lt with
-  | nil_term => nil
-  | cons_term hd tl =>
-    (term_semantics ctxt_var ctxt_fct hd)::(list_term_semantics ctxt_var ctxt_fct tl)
+  | var s => 1
+  | fn s l => 1 + sum_list_nat (map term_measure l)
   end.
 
-Fixpoint term_free_vars (t: term) : list string :=
+Lemma term_measure_elt: forall s l x,
+    In x l ->
+    term_measure x < term_measure (fn s l).
+intro; induction l; intuition.
+inversion H.
+simpl; simpl in IHl.
+inversion_clear H.
+subst a; omega.
+generalize (IHl x H0); intros; auto.
+omega.
+Qed.
+
+Require Import Coq.Program.Wf.
+
+Program Fixpoint term_recursion
+        (P: term -> Type)
+        (P_var: forall s: string, P (var s))
+        (P_fn: forall (s: string) (l: list term),
+            (forall x, In x l -> P x) -> P (fn s l))
+        (t: term) { measure (term_measure t) } : P t :=
   match t with
-  | var s => s::nil
-  | fct f ts => list_term_free_vars ts
-  end
-with
-list_term_free_vars (ts: list_term): list string :=
-  match ts with
-  | nil_term => nil
-  | cons_term hd tl =>
-    term_free_vars hd ++ list_term_free_vars tl
+  | var s => P_var s
+  | fn s l => P_fn s l (fun x H => term_recursion P P_var P_fn x)
   end.
+Next Obligation.  
+apply term_measure_elt; auto.
+Qed.
 
-Program Fixpoint term_semantics_free_vars
+(* this is a couple simple rewriting rule that one could use for simplification in lemmas *)
+Lemma term_recursion_var P P_var P_fn: forall s,
+    term_recursion P P_var P_fn (var s) = P_var s.
+auto.
+Qed.
+
+Lemma term_recursion_fn P P_var P_fn: forall s l,
+    term_recursion P P_var P_fn (fn s l) = P_fn s l (fun x H => term_recursion P P_var P_fn x).
+  intros.
+  unfold term_recursion.
+  unfold term_recursion_func.
+  rewrite WfExtensionality.fix_sub_eq_ext.
+  simpl.
+  auto.
+Qed.
+
+(* we are going to need a map variant *)
+Program Fixpoint map_term {A: Set} (l: list term) (P: forall x: term, In x l -> A) { struct l }: list A :=
+  match l with
+  | nil => nil
+  | hd::tl => (P hd _)::(@map_term A tl (fun x H => P x _))
+  end.
+Next Obligation.
+  intuition.
+Qed.
+Next Obligation.
+  intuition.
+Qed.
+
+(* specialization of the term_recursion rewriting rule *)
+Lemma term_recursion_map_term_var {A: Set} (f_var: string -> A) (f_fn: string -> list A -> A): forall s,
+    term_recursion (fun t => A) f_var (fun s l H => f_fn s (map_term l H)) (var s) =
+    f_var s.
+  intros.
+  rewrite term_recursion_var.
+  auto.
+Qed.
+  
+  Lemma term_recursion_map_term_fn {A: Set} (f_var: string -> A) (f_fn: string -> list A -> A): forall s l,
+    term_recursion (fun t => A) f_var (fun s l H => f_fn s (map_term l H)) (fn s l) =
+    f_fn s (map (term_recursion (fun t => A) f_var (fun s l H => f_fn s (map_term l H))) l).
+  intros.
+  rewrite term_recursion_fn.
+  f_equal.
+  generalize l; clear l.
+  induction l; simpl; intros; intuition.
+  f_equal.
+  rewrite <- IHl.
+  auto.
+Qed.
+  
+(**)
+
+Program Fixpoint list_dec {A: Set} (l1: list A) (A_dec: forall a1, In a1 l1 -> forall a2, { a1 = a2 } + { a1 <> a2 }) (l2: list A) { struct l1 }: { l1 = l2 } + { l1 <> l2 } :=
+  match l1 with
+  | nil => _
+  | hd::tl => _ (@list_dec A tl _)
+  end.
+Next Obligation.
+  destruct l2; simpl; auto.
+  right; intro H; inversion H.
+Defined.
+Next Obligation.
+  destruct l2 ;simpl; auto.
+  right; intro H; inversion H.
+  assert (In hd (hd::tl)) by intuition.
+  generalize (A_dec _ H a); intro H1; inversion_clear H1.
+  subst a; generalize (x l2); intro H0; inversion_clear H0.
+  subst l2; left; intuition.
+  right; simpl; injection.
+  auto.
+  right; injection; intuition.
+Defined.
+Next Obligation.
+  intuition.
+Defined.
+
+Program Definition term_eq_dec (t1: term) : forall t2, { t1 = t2 } + { t1 <> t2 }:=
+  term_recursion (fun t => forall t2, { t = t2 } + { t <> t2 }) _ _ t1.
+Next Obligation.
+  destruct t2.
+  generalize (string_dec s s0); intro H0; inversion_clear H0.
+  subst; intuition.
+  right; injection; intuition.
+  right; intro H0; inversion_clear H0.
+Defined.
+Next Obligation.
+  destruct t2.
+  right; intro H0; inversion_clear H0.
+  generalize (string_dec s s0); intro H0; inversion_clear H0.
+  generalize (list_dec l H l0); intro H0; inversion_clear H0.
+  subst s l; intuition.
+  right; injection; intuition.
+  right; injection; intuition.
+Defined.
+
+(**)
+
+
+Definition term_semantics
+           {Value: InhabitedType}
+           (ctxt_var: string -> Value)
+           (ctxt_fn: string -> list Value -> Value)
+           (t: term): Value :=
+  term_recursion (fun t => Value) ctxt_var (fun s l H => ctxt_fn s (map_term l H)) t.
+
+Lemma term_semantics_var
+      {Value: InhabitedType}
+      (ctxt_var: string -> Value)
+      (ctxt_fn: string -> list Value -> Value): forall s,
+    term_semantics ctxt_var ctxt_fn (var s) =
+    ctxt_var s.
+  intros.
+  unfold term_semantics.
+  apply term_recursion_map_term_var.
+Qed.
+
+
+Lemma term_semantics_fn
+      {Value: InhabitedType}
+      (ctxt_var: string -> Value)
+      (ctxt_fn: string -> list Value -> Value): forall s l,
+    term_semantics ctxt_var ctxt_fn (fn s l) =
+    ctxt_fn s (map (term_semantics ctxt_var ctxt_fn) l).
+  intros.
+  unfold term_semantics.
+  apply term_recursion_map_term_fn.
+Qed.
+
+Definition term_free_vars (t: term): list string :=
+  term_recursion (fun t => list string) (fun s => s::nil) (fun s l H => concat (map_term l H)) t.
+
+Lemma term_free_vars_fn: forall s l,
+    term_free_vars (fn s l) = concat (map term_free_vars l).
+  intros.
+  unfold term_free_vars.
+  apply term_recursion_map_term_fn with (f_fn := fun s l => concat l).
+Qed.
+
+Program Definition term_semantics_free_vars
         {Value: InhabitedType}
         (t: term)
-        (ctxt_fct: string -> list Value -> Value)
+        (ctxt_fn: string -> list Value -> Value)
         (ctxt_var1: string -> Value)
-        (ctxt_var2: string -> Value)
-        (Hyp: forall s, List.In s (term_free_vars t) -> ctxt_var1 s = ctxt_var2 s):
-  @term_semantics Value ctxt_var1 ctxt_fct t = @term_semantics Value ctxt_var2 ctxt_fct t :=
-  match t with
-  | var s => _
-  | fct f lt =>
-    let H := @list_term_semantics_free_vars Value lt ctxt_fct ctxt_var1 ctxt_var2 _ in
-    _ H
-  end
-with
-list_term_semantics_free_vars
-  {Value: InhabitedType}
-  (lt: list_term)
-  (ctxt_fct: string -> list Value -> Value)
-  (ctxt_var1: string -> Value)
-  (ctxt_var2: string -> Value)
-  (Hyp: forall s, List.In s (list_term_free_vars lt) -> ctxt_var1 s = ctxt_var2 s):
-  @list_term_semantics Value ctxt_var1 ctxt_fct lt = @list_term_semantics Value ctxt_var2 ctxt_fct lt :=
-  match lt with
-  | nil_term => _
-  | cons_term hd tl =>
-    let H1 := @term_semantics_free_vars Value hd ctxt_fct ctxt_var1 ctxt_var2 _ in
-    let H2 := @list_term_semantics_free_vars Value tl ctxt_fct ctxt_var1 ctxt_var2 _ in
-    _ H1 H2
-  end.
+        (ctxt_var2: string -> Value):
+        (forall s, List.In s (term_free_vars t) -> ctxt_var1 s = ctxt_var2 s) ->
+  @term_semantics Value ctxt_var1 ctxt_fn t = @term_semantics Value ctxt_var2 ctxt_fn t :=
+  term_recursion (fun t =>
+                    (forall s, List.In s (term_free_vars t) -> ctxt_var1 s = ctxt_var2 s) ->
+                    @term_semantics Value ctxt_var1 ctxt_fn t = @term_semantics Value ctxt_var2 ctxt_fn t) _ _ t.
 Next Obligation.
-  apply Hyp; simpl; apply List.in_or_app; auto.
-Defined.
+cut (ctxt_var1 s = ctxt_var2 s); intuition.
+Qed.
 Next Obligation.
-  apply Hyp; simpl; apply List.in_or_app; auto.
-Defined.
-Next Obligation.
-  apply Hyp; simpl; auto.
-Defined.
-
+  do 2 rewrite term_semantics_fn.
+  f_equal.
+  apply map_ext_in; intros.
+  apply H; auto.
+  intros.
+  apply H0.
+  rewrite term_free_vars_fn.
+  rewrite <- flat_map_concat_map; rewrite in_flat_map; exists a; auto.
+Qed.
+  
 (*****************************************)
 
-Inductive formula : Set :=
-| T: formula
-| F: formula
-| Atom: string -> list_term -> formula
+(* this is just really to match the ocaml code on extraction *)
+
+Inductive fol: Set :=
+  | R: string -> list term -> fol.
+
+Inductive formula {A: Set}: Set :=
+| True: formula
+| False: formula
+| Atom: A -> formula
 | Eq: term -> term -> formula
 | Not: formula -> formula
 | And: formula -> formula -> formula
@@ -181,21 +253,14 @@ Inductive formula : Set :=
 | Exists: string -> formula -> formula
 .
 
-Definition list_dec:
-  forall {A: Set}
-         (A_dec: forall (a1 a2: A), {a1 = a2} + {a1 <> a2})
-         (l1 l2: list A),
-    {l1 = l2} + {l1 <> l2}.
-decide equality.
-Defined.
 
-
-Definition formula_dec: forall (f1 f2: formula), {f1 = f2} + {f1 <> f2}.
+Definition formula_dec: forall (f1 f2: @formula fol), {f1 = f2} + {f1 <> f2}.
   decide equality.
-  apply list_term_dec; apply term_dec.
+  decide equality.
+  apply List.list_eq_dec; apply term_eq_dec.
   apply string_dec.
-  apply term_dec.
-  apply term_dec.
+  apply term_eq_dec.
+  apply term_eq_dec.
   apply string_dec.
   apply string_dec.
 Defined.
@@ -203,42 +268,42 @@ Defined.
 Fixpoint formula_semantics 
          {Value: InhabitedType}
          (ctxt_var: string -> Value)
-         (ctxt_fct: string -> list Value -> Value)
+         (ctxt_fn: string -> list Value -> Value)
          (ctxt_pred: string -> list Value -> Prop)
-         (f: formula) : Prop :=
+         (f: @formula fol) : Prop :=
   match f with
-  | T => True
-  | F => False
-  | Atom P args => ctxt_pred P (list_term_semantics ctxt_var ctxt_fct args)
-  | Eq t1 t2 => term_semantics ctxt_var ctxt_fct t1 = term_semantics ctxt_var ctxt_fct t2
-  | Not f => ~ (formula_semantics ctxt_var ctxt_fct ctxt_pred f)
-  | And f1 f2 => (formula_semantics ctxt_var ctxt_fct ctxt_pred f1) /\ (formula_semantics ctxt_var ctxt_fct ctxt_pred f2) 
-  | Or f1 f2 => (formula_semantics ctxt_var ctxt_fct ctxt_pred f1) \/ (formula_semantics ctxt_var ctxt_fct ctxt_pred f2) 
-  | Imp f1 f2 => (formula_semantics ctxt_var ctxt_fct ctxt_pred f1) -> (formula_semantics ctxt_var ctxt_fct ctxt_pred f2) 
-  | Iff f1 f2 => (formula_semantics ctxt_var ctxt_fct ctxt_pred f1) <-> (formula_semantics ctxt_var ctxt_fct ctxt_pred f2)
+  | True => Logic.True
+  | False => Logic.False
+  | Atom (R P args) => ctxt_pred P (map (term_semantics ctxt_var ctxt_fn) args)
+  | Eq t1 t2 => term_semantics ctxt_var ctxt_fn t1 = term_semantics ctxt_var ctxt_fn t2
+  | Not f => ~ (formula_semantics ctxt_var ctxt_fn ctxt_pred f)
+  | And f1 f2 => (formula_semantics ctxt_var ctxt_fn ctxt_pred f1) /\ (formula_semantics ctxt_var ctxt_fn ctxt_pred f2) 
+  | Or f1 f2 => (formula_semantics ctxt_var ctxt_fn ctxt_pred f1) \/ (formula_semantics ctxt_var ctxt_fn ctxt_pred f2) 
+  | Imp f1 f2 => (formula_semantics ctxt_var ctxt_fn ctxt_pred f1) -> (formula_semantics ctxt_var ctxt_fn ctxt_pred f2) 
+  | Iff f1 f2 => (formula_semantics ctxt_var ctxt_fn ctxt_pred f1) <-> (formula_semantics ctxt_var ctxt_fn ctxt_pred f2)
   | Forall x f => forall (v: Value),
       formula_semantics
         (fun y => match string_dec x y with | left _ => v | right _ => ctxt_var y end)
-        ctxt_fct ctxt_pred f
+        ctxt_fn ctxt_pred f
   | Exists x f => exists (v: Value),
       formula_semantics
         (fun y => match string_dec x y with | left _ => v | right _ => ctxt_var y end)
-        ctxt_fct ctxt_pred f
+        ctxt_fn ctxt_pred f
   end.
 
 Axiom classical_formula:
   forall {Value: InhabitedType}
          (ctxt_var: string -> Value)
-         (ctxt_fct: string -> list Value -> Value)
+         (ctxt_fn: string -> list Value -> Value)
          (ctxt_pred: string -> list Value -> Prop)
          (f: formula),
-    (formula_semantics ctxt_var ctxt_fct ctxt_pred f) \/ ~ (formula_semantics ctxt_var ctxt_fct ctxt_pred f).
+    (formula_semantics ctxt_var ctxt_fn ctxt_pred f) \/ ~ (formula_semantics ctxt_var ctxt_fn ctxt_pred f).
 
 Fixpoint formula_free_vars (f: formula) : list string :=
     match f with
-  | T => nil
-  | F => nil
-  | Atom P args => list_term_free_vars args
+  | True => nil
+  | False => nil
+  | Atom (R P args) => concat (map term_free_vars args)
   | Eq t1 t2 => term_free_vars t1 ++ term_free_vars t2
   | Not f => formula_free_vars f
   | And f1 f2 => formula_free_vars f1 ++ formula_free_vars f2
@@ -248,26 +313,43 @@ Fixpoint formula_free_vars (f: formula) : list string :=
   | Forall x f => List.remove string_dec x (formula_free_vars f)
   | Exists x f => List.remove string_dec x (formula_free_vars f)
   end.
+  
+Lemma remove_In_diff: forall {A: Set} H
+                             (l: list A) (x x0: A), x <> x0 -> List.In x l -> List.In x (@List.remove _ H x0 l).
+  do 2 intro.
+  induction l; simpl; intros; auto.
+  inversion_clear H1.
+  subst x.
+  destruct (H x0 a); intuition.
+  subst a.
+  intuition.
+  destruct (H x0 a); intuition.
+Qed.
 
 Lemma formula_semantics_free_vars:
   forall
       {Value: InhabitedType}
       (f: formula)
-      (ctxt_fct: string -> list Value -> Value)
+      (ctxt_fn: string -> list Value -> Value)
       (ctxt_pred: string -> list Value -> Prop)
       (ctxt_var1: string -> Value)
       (ctxt_var2: string -> Value)
       (Hyp: forall s, List.In s (formula_free_vars f) -> ctxt_var1 s = ctxt_var2 s),
-  (formula_semantics ctxt_var1 ctxt_fct ctxt_pred f) <-> (formula_semantics ctxt_var2 ctxt_fct ctxt_pred f).
+  (formula_semantics ctxt_var1 ctxt_fn ctxt_pred f) <-> (formula_semantics ctxt_var2 ctxt_fn ctxt_pred f).
 
   induction f; simpl; intros.
 
   intuition.
   intuition.
 
-  rewrite list_term_semantics_free_vars with (ctxt_var4 := ctxt_var2).
+  destruct a.
+  cut (map (term_semantics ctxt_var1 ctxt_fn) l = map (term_semantics ctxt_var2 ctxt_fn) l).
+  intro H; rewrite H; split; auto.
+  apply map_ext_in; intros.
+  eapply term_semantics_free_vars.
   intuition.
-  auto.
+  eapply Hyp.
+  rewrite <- flat_map_concat_map; rewrite in_flat_map; exists a; auto.
 
   rewrite term_semantics_free_vars with (ctxt_var3 := ctxt_var1) (ctxt_var4 := ctxt_var2).
   rewrite term_semantics_free_vars with (ctxt_var3 := ctxt_var1) (ctxt_var4 := ctxt_var2).
@@ -300,18 +382,6 @@ Lemma formula_semantics_free_vars:
   intuition.
   intuition.
   intuition.
-  
-  Lemma remove_In_diff: forall {A: Set} H
-                               (l: list A) (x x0: A), x <> x0 -> List.In x l -> List.In x (@List.remove _ H x0 l).
-    do 2 intro.
-    induction l; simpl; intros; auto.
-    inversion_clear H1.
-    subst x.
-    destruct (H x0 a); intuition.
-    subst a.
-    intuition.
-    destruct (H x0 a); intuition.
-  Qed.
 
   split; intros; intuition.
   rewrite IHf with (ctxt_var2 := (fun y : string => if string_dec s y then v else ctxt_var1 y)); auto.
@@ -348,15 +418,15 @@ Qed.
 Module Type ProofSystem.
 
   Parameter Thm: Set.
-  Parameter concl: Thm -> formula.
+  Parameter concl: Thm -> @formula fol.
 
   Parameter proof:
     forall (thm: Thm)
            {Value: InhabitedType}
            (ctxt_var: string -> Value)
-           (ctxt_fct: string -> list Value -> Value)
+           (ctxt_fn: string -> list Value -> Value)
            (ctxt_pred: string -> list Value -> Prop),
-      @formula_semantics Value ctxt_var ctxt_fct ctxt_pred (concl thm).
+      @formula_semantics Value ctxt_var ctxt_fn ctxt_pred (concl thm).
 
   (*  if |- p ==> q and |- p then |- q                                         *)
   Parameter modus_ponens: Thm -> Thm -> Thm.
@@ -365,19 +435,19 @@ Module Type ProofSystem.
   Parameter gen: string -> Thm -> Thm.
   
   (*  |- p ==> (q ==> p)                                                       *)
-  Parameter axiom_addimp: formula -> formula -> Thm.
+  Parameter axiom_addimp: @formula fol -> @formula fol -> Thm.
   
   (*  |- (p ==> q ==> r) ==> (p ==> q) ==> (p ==> r)                           *)
-  Parameter axiom_distribimp: formula -> formula -> formula -> Thm.
+  Parameter axiom_distribimp: @formula fol -> @formula fol -> @formula fol -> Thm.
   
   (*  |- ((p ==> false) ==> false) ==> p                                       *)
-  Parameter axiom_doubleneg: formula -> Thm.
+  Parameter axiom_doubleneg: @formula fol -> Thm.
   
   (*  |- (forall x. p ==> q) ==> (forall x. p) ==> (forall x. q)               *)
-  Parameter axiom_allimp: string -> formula -> formula -> Thm.
+  Parameter axiom_allimp: string -> @formula fol -> @formula fol -> Thm.
     
   (*  |- p ==> forall x. p                            [x not free in p]        *)
-  Parameter axiom_impall: string -> formula -> Thm.
+  Parameter axiom_impall: string -> @formula fol -> Thm.
   
   (*  |- exists x. x = t                              [x not free in t]        *)
   Parameter axiom_existseq: string -> term -> Thm.
@@ -386,34 +456,34 @@ Module Type ProofSystem.
   Parameter axiom_eqrefl: term -> Thm.
   
   (*  |- s1 = t1 ==> ... ==> sn = tn ==> f(s1,..,sn) = f(t1,..,tn)             *)
-  Parameter axiom_funcong: string -> list_term -> list_term -> Thm.
+  Parameter axiom_funcong: string -> list term -> list term -> Thm.
   
   (*  |- s1 = t1 ==> ... ==> sn = tn ==> P(s1,..,sn) ==> P(t1,..,tn)           *)
-  Parameter axiom_predcong: string -> list_term -> list_term -> Thm.
+  Parameter axiom_predcong: string -> list term -> list term -> Thm.
   
   (*  |- (p <=> q) ==> p ==> q                                                 *)
-  Parameter axiom_iffimp1: formula -> formula -> Thm.
+  Parameter axiom_iffimp1: @formula fol -> @formula fol -> Thm.
   
   (*  |- (p <=> q) ==> q ==> p                                                 *)
-  Parameter axiom_iffimp2: formula -> formula -> Thm.
+  Parameter axiom_iffimp2: @formula fol -> @formula fol -> Thm.
 
   (*  |- (p ==> q) ==> (q ==> p) ==> (p <=> q)                                 *)
-  Parameter axiom_impiff: formula -> formula -> Thm.
+  Parameter axiom_impiff: @formula fol -> @formula fol -> Thm.
 
   (*  |- true <=> (false ==> false)                                            *)
   Parameter axiom_true: Thm.
   
   (*  |- ~p <=> (p ==> false)                                                  *)
-  Parameter axiom_not: formula -> Thm.
+  Parameter axiom_not: @formula fol -> Thm.
   
   (*  |- p /\ q <=> (p ==> q ==> false) ==> false                              *)
-  Parameter axiom_and: formula -> formula -> Thm.
+  Parameter axiom_and: @formula fol -> @formula fol -> Thm.
   
   (*  |- p \/ q <=> ~(~p /\ ~q)                                                *)
-  Parameter axiom_or: formula -> formula -> Thm.
+  Parameter axiom_or: @formula fol -> @formula fol -> Thm.
 
   (*  |- (exists x. p) <=> ~(forall x. ~p)                                     *)
-  Parameter axiom_exists: string -> formula -> Thm.
+  Parameter axiom_exists: string -> @formula fol -> Thm.
 
 End ProofSystem.
 
@@ -424,14 +494,14 @@ Module Proven: ProofSystem.
                        proof: forall 
                            {Value: InhabitedType}
                            (ctxt_var: string -> Value)
-                           (ctxt_fct: string -> list Value -> Value)
+                           (ctxt_fn: string -> list Value -> Value)
                            (ctxt_pred: string -> list Value -> Prop),
-                           formula_semantics ctxt_var ctxt_fct ctxt_pred concl;
+                           formula_semantics ctxt_var ctxt_fn ctxt_pred concl;
                        }.
 
   Definition Thm := Impl.
 
-  Program Definition T_Thm := mkImpl T _.
+  Program Definition T_Thm := mkImpl True _.
   
   (*  if |- p ==> q and |- p then |- q                                         *)
   Program Definition modus_ponens (thm1 thm2: Thm): Thm :=
@@ -444,8 +514,8 @@ Module Proven: ProofSystem.
     | _ => T_Thm
     end.
   Next Obligation.
-    generalize (@proof thm1 Value ctxt_var ctxt_fct ctxt_pred); intros.
-    generalize (@proof thm2 Value ctxt_var ctxt_fct ctxt_pred); intros.
+    generalize (@proof thm1 Value ctxt_var ctxt_fn ctxt_pred); intros.
+    generalize (@proof thm2 Value ctxt_var ctxt_fn ctxt_pred); intros.
     rewrite <- Heq_anonymous0 in H.
     simpl in H.
     intuition.
@@ -465,9 +535,9 @@ Module Proven: ProofSystem.
     mkImpl (Imp (Imp p (Imp q r)) (Imp (Imp p q) (Imp p r))) _.
   
   (*  |- ((p ==> false) ==> false) ==> p                                       *)
-  Program Definition axiom_doubleneg (p: formula): Thm := mkImpl (Imp (Imp (Imp p F) F) p) _.
+  Program Definition axiom_doubleneg (p: formula): Thm := mkImpl (Imp (Imp (Imp p False) False) p) _.
   Next Obligation.
-    generalize (classical_formula ctxt_var ctxt_fct ctxt_pred p); intro H0; inversion_clear H0; auto.
+    generalize (classical_formula ctxt_var ctxt_fn ctxt_pred p); intro H0; inversion_clear H0; auto.
     intuition.
   Qed.  
   
@@ -502,67 +572,67 @@ Module Proven: ProofSystem.
     | right _ => mkImpl (Exists x (Eq (var x) t)) _
     end.
   Next Obligation.
-    exists (term_semantics ctxt_var ctxt_fct t).
-    destruct (string_dec x x).
-    apply term_semantics_free_vars; intros.
+    exists (term_semantics ctxt_var ctxt_fn t).
+    rewrite term_semantics_var.
+    destruct (string_dec x x); [ idtac | intuition ].
+    eapply term_semantics_free_vars; intros.
     destruct (string_dec x s).
     subst s; contradiction.
     auto.
-    intuition.
   Qed.
 
   (*  |- t = t                                                                 *)
   Program Definition axiom_eqrefl (t: term): Thm := mkImpl (Eq t t) _.    
   
   (*  |- s1 = t1 ==> ... ==> sn = tn ==> f(s1,..,sn) = f(t1,..,tn)             *)
-  Fixpoint list_term_prefix (l1 l2: list_term): list_term :=
+  Fixpoint list_term_prefix (l1 l2: list term): list term :=
     match l2 with
-    | nil_term => l1
-    | cons_term hd2 tl2 =>
+    | nil  => l1
+    | hd2::tl2 =>
       match l1 with
-      | nil_term => nil_term
-      | cons_term hd1 tl1 =>
-        cons_term hd2 (list_term_prefix tl1 tl2)
+      | nil => nil
+      | hd1::tl1 =>
+        hd2::(list_term_prefix tl1 tl2)
       end
     end.
 
   Lemma list_term_prefix_nil_right: forall l,
-      list_term_prefix l nil_term = l.
+      list_term_prefix l nil = l.
     induction l; simpl; auto.
   Qed.
 
-  Fixpoint zip_list_term (l1 l2: list_term): list (term * term) :=
+  Fixpoint zip_list_term (l1 l2: list term): list (term * term) :=
     match l1, l2 with
-    | cons_term hd1 tl1, cons_term hd2 tl2 =>
+    | hd1::tl1, hd2::tl2 =>
       (hd1, hd2)::(zip_list_term tl1 tl2)
     | _, _ => nil
     end.
 
   Lemma zip_list_term_nil_left: forall l,
-      zip_list_term nil_term l = nil.
+      zip_list_term nil l = nil.
     intuition.
   Qed.
 
   Lemma zip_list_term_nil_right: forall l,
-      zip_list_term l nil_term = nil.
+      zip_list_term l nil = nil.
     induction l; simpl; intuition.
   Qed.
 
   Lemma list_term_semantics_eq_term:
     forall {Value: InhabitedType}
            (ctxt_var: string -> Value)
-           (ctxt_fct: string -> list Value -> Value),
+           (ctxt_fn: string -> list Value -> Value),
     forall rhs lhs,
              (forall x, List.In x (zip_list_term lhs rhs) ->
                         let (x1, x2) := x in
-                        @term_semantics Value ctxt_var ctxt_fct x1 = @term_semantics Value ctxt_var ctxt_fct x2) ->
-             @list_term_semantics Value ctxt_var ctxt_fct lhs =
-             @list_term_semantics Value ctxt_var ctxt_fct (list_term_prefix lhs rhs).
+                        @term_semantics Value ctxt_var ctxt_fn x1 = @term_semantics Value ctxt_var ctxt_fn x2) ->
+             map (@term_semantics Value ctxt_var ctxt_fn) lhs =
+             map (@term_semantics Value ctxt_var ctxt_fn) (list_term_prefix lhs rhs).
     do 4 intro.
     induction rhs; simpl; intros; auto.
     rewrite list_term_prefix_nil_right; auto.
     destruct lhs; auto.
-    simpl; simpl in H; rewrite (H (t0, t)).
+    simpl; simpl in H; rewrite (H (t, a)).
     apply f_equal.
     apply IHrhs.
     intros.
@@ -574,55 +644,56 @@ Qed.
   Lemma fun_congruence_eq_term:
     forall {Value: InhabitedType}
            (ctxt_var: string -> Value)
-           (ctxt_fct: string -> list Value -> Value)
+           (ctxt_fn: string -> list Value -> Value)
            (ctxt_pred: string -> list Value -> Prop),
     forall f rhs lhs,
              (forall x, List.In x (zip_list_term lhs rhs) ->
                         let (x1, x2) := x in
-                        @formula_semantics Value ctxt_var ctxt_fct ctxt_pred (Eq x1 x2)
+                        @formula_semantics Value ctxt_var ctxt_fn ctxt_pred (Eq x1 x2)
                         ) ->
-             @formula_semantics Value ctxt_var ctxt_fct ctxt_pred (Eq (fct f lhs) (fct f (list_term_prefix lhs rhs))).
+             @formula_semantics Value ctxt_var ctxt_fn ctxt_pred (Eq (fn f lhs) (fn f (list_term_prefix lhs rhs))).
     simpl; intros.
+    do 2 rewrite term_semantics_fn.
     rewrite <- list_term_semantics_eq_term; auto.
   Qed.
 
   Lemma pred_congruence_eq_term:
     forall {Value: InhabitedType}
            (ctxt_var: string -> Value)
-           (ctxt_fct: string -> list Value -> Value)
+           (ctxt_fn: string -> list Value -> Value)
            (ctxt_pred: string -> list Value -> Prop),
     forall P rhs lhs,
              (forall x, List.In x (zip_list_term lhs rhs) ->
                         let (x1, x2) := x in
-                        @formula_semantics Value ctxt_var ctxt_fct ctxt_pred (Eq x1 x2)
+                        @formula_semantics Value ctxt_var ctxt_fn ctxt_pred (Eq x1 x2)
                         ) ->
-             @formula_semantics Value ctxt_var ctxt_fct ctxt_pred (
+             @formula_semantics Value ctxt_var ctxt_fn ctxt_pred (
                                   Imp
-                                    (Atom P lhs)
-                                    (Atom P (list_term_prefix lhs rhs))
+                                    (Atom (R P lhs))
+                                    (Atom (R P (list_term_prefix lhs rhs)))
                                 ).
     simpl; intros.
     rewrite <- list_term_semantics_eq_term; auto.
   Qed.
   
-  Fixpoint build_conj (fs: list formula) : formula :=
+  Fixpoint build_conj (fs: list (@formula fol)) : formula :=
     match fs with
-    | nil => T
+    | nil => True
     | hd::tl => And hd (build_conj tl)
     end.
 
   Lemma build_conj_sem:
     forall {Value: InhabitedType}
            (ctxt_var: string -> Value)
-           (ctxt_fct: string -> list Value -> Value)
+           (ctxt_fn: string -> list Value -> Value)
            (ctxt_pred: string -> list Value -> Prop),
     forall l,
-      @formula_semantics Value ctxt_var ctxt_fct ctxt_pred (
+      @formula_semantics Value ctxt_var ctxt_fn ctxt_pred (
                            build_conj (List.map (fun x: (term * term) => let (x1, x2) := x in Eq x1 x2) l)
                          ) <->
       (forall x, List.In x l ->
                         let (x1, x2) := x in
-                        @formula_semantics Value ctxt_var ctxt_fct ctxt_pred (Eq x1 x2)
+                        @formula_semantics Value ctxt_var ctxt_fn ctxt_pred (Eq x1 x2)
                         ).
     do 4 intro.
     induction l; simpl; intros.
@@ -646,7 +717,7 @@ Qed.
     destruct x; intuition.
 Qed.
 
-  Fixpoint build_imp (fs: list formula) (ccl: formula): formula :=
+  Fixpoint build_imp (fs: list (@formula fol)) (ccl: formula): formula :=
     match fs with
     | nil => ccl
     |hd::tl => Imp hd (build_imp tl ccl)
@@ -655,13 +726,13 @@ Qed.
   Lemma build_conj_imp_equiv:
     forall {Value: InhabitedType}
            (ctxt_var: string -> Value)
-           (ctxt_fct: string -> list Value -> Value)
+           (ctxt_fn: string -> list Value -> Value)
            (ctxt_pred: string -> list Value -> Prop),
     forall fs ccl,
-      @formula_semantics Value ctxt_var ctxt_fct ctxt_pred (
+      @formula_semantics Value ctxt_var ctxt_fn ctxt_pred (
                            Imp (build_conj fs) ccl
                          ) <->
-      @formula_semantics Value ctxt_var ctxt_fct ctxt_pred (
+      @formula_semantics Value ctxt_var ctxt_fn ctxt_pred (
                            build_imp fs ccl
                          ).
     do 4 intro; induction fs; split; simpl; intros.
@@ -675,22 +746,22 @@ Qed.
     intuition.
   Qed.    
 
-  Program Definition axiom_funcong_aux (f: string) (lhs rhs: list_term) : Thm :=
+  Program Definition axiom_funcong_aux (f: string) (lhs rhs: list term) : Thm :=
     mkImpl (
         Imp
           (build_conj (List.map (fun x: (term * term) => let (x1, x2) := x in Eq x1 x2) (zip_list_term lhs rhs)))
-          (Eq (fct f lhs) (fct f (list_term_prefix lhs rhs)))
+          (Eq (fn f lhs) (fn f (list_term_prefix lhs rhs)))
       ) _.
   Next Obligation.
-    apply (fun_congruence_eq_term ctxt_var ctxt_fct ctxt_pred).
+    apply (fun_congruence_eq_term ctxt_var ctxt_fn ctxt_pred).
     rewrite <- build_conj_sem; auto.
   Qed.
 
-  Program Definition axiom_funcong (f: string) (lhs rhs: list_term) : Thm :=
+  Program Definition axiom_funcong (f: string) (lhs rhs: list term) : Thm :=
     mkImpl (
         build_imp
           (List.map (fun x: (term * term) => let (x1, x2) := x in Eq x1 x2) (zip_list_term lhs rhs))
-          (Eq (fct f lhs) (fct f (list_term_prefix lhs rhs)))
+          (Eq (fn f lhs) (fn f (list_term_prefix lhs rhs)))
       ) _.
   Next Obligation.
     rewrite <- build_conj_imp_equiv.
@@ -698,22 +769,22 @@ Qed.
   Qed.
   
   (*  |- s1 = t1 ==> ... ==> sn = tn ==> P(s1,..,sn) ==> P(t1,..,tn)           *)
-  Program Definition axiom_predcong_aux (P: string) (lhs rhs: list_term) : Thm :=
+  Program Definition axiom_predcong_aux (P: string) (lhs rhs: list term) : Thm :=
     mkImpl (
         Imp
           (build_conj (List.map (fun x: (term * term) => let (x1, x2) := x in Eq x1 x2) (zip_list_term lhs rhs)))
-          (Imp (Atom P lhs) (Atom P (list_term_prefix lhs rhs)))
+          (Imp (Atom (R P lhs)) (Atom (R P (list_term_prefix lhs rhs))))
       ) _.
   Next Obligation.
-    apply (pred_congruence_eq_term ctxt_var ctxt_fct ctxt_pred).
+    apply (pred_congruence_eq_term ctxt_var ctxt_fn ctxt_pred).
     rewrite <- build_conj_sem; auto.
     auto.
   Qed.
 
-  Program Definition axiom_predcong (P: string) (lhs rhs: list_term) : Thm :=
+  Program Definition axiom_predcong (P: string) (lhs rhs: list term) : Thm :=
     mkImpl (
         build_imp (List.map (fun x: (term * term) => let (x1, x2) := x in Eq x1 x2) (zip_list_term lhs rhs))
-           (Imp (Atom P lhs) (Atom P (list_term_prefix lhs rhs)))
+           (Imp (Atom (R P lhs)) (Atom (R P (list_term_prefix lhs rhs))))
       ) _.
   Next Obligation.
     rewrite <- build_conj_imp_equiv.
@@ -757,13 +828,13 @@ Qed.
   Qed.
   
   (*  |- true <=> (false ==> false)                                            *)
-  Program Definition axiom_true: Thm := mkImpl (Iff T (Imp F F)) _.
+  Program Definition axiom_true: Thm := mkImpl (Iff True (Imp False False)) _.
   Next Obligation.
     split; auto.
   Qed.
   
   (*  |- ~p <=> (p ==> false)                                                  *)
-  Program Definition axiom_not (p: formula): Thm := mkImpl (Iff (Not p) (Imp p F)) _.
+  Program Definition axiom_not (p: formula): Thm := mkImpl (Iff (Not p) (Imp p False)) _.
   Next Obligation.
     split; auto.
   Qed.  
@@ -773,13 +844,13 @@ Qed.
     mkImpl (
         Iff
           (And p q)
-          (Imp (Imp p (Imp q F)) F)
+          (Imp (Imp p (Imp q False)) False)
       ) _.
   Next Obligation.
     split; intros; auto.
     intuition.
-    generalize (classical_formula ctxt_var ctxt_fct ctxt_pred p); intro H1.
-    generalize (classical_formula ctxt_var ctxt_fct ctxt_pred q); intro H2.
+    generalize (classical_formula ctxt_var ctxt_fn ctxt_pred p); intro H1.
+    generalize (classical_formula ctxt_var ctxt_fn ctxt_pred q); intro H2.
     intuition.
   Qed.
         
@@ -793,8 +864,8 @@ Qed.
   Next Obligation.
     split; intros; auto.
     intuition.
-    generalize (classical_formula ctxt_var ctxt_fct ctxt_pred p); intro H1.
-    generalize (classical_formula ctxt_var ctxt_fct ctxt_pred q); intro H2.
+    generalize (classical_formula ctxt_var ctxt_fn ctxt_pred p); intro H1.
+    generalize (classical_formula ctxt_var ctxt_fn ctxt_pred q); intro H2.
     intuition.
   Qed.
 
@@ -811,9 +882,9 @@ Qed.
     inversion_clear H.
     generalize (H0 x0).
     contradiction.
-    generalize (classical_formula ctxt_var ctxt_fct ctxt_pred (Exists x p)); simpl; intro H1.
+    generalize (classical_formula ctxt_var ctxt_fn ctxt_pred (Exists x p)); simpl; intro H1.
     inversion_clear H1; auto.
-    assert False.
+    assert Logic.False.
     apply H.
     intros; red; intros.
     apply H0.
@@ -823,6 +894,12 @@ Qed.
 
 End Proven.
 
+
+Require Import Coq.extraction.ExtrOcamlString.
+Require Import Coq.extraction.ExtrOcamlBasic.
+Require Import ExtrOcamlNatBigInt.
+
+Extraction "harrison.ml" Proven.
 
 
 
